\documentclass[UTF8,a4paper,notitlepage,openany,plain,final]{ctexbook}
    \author{王亚}
    \title{App运营指南}
    \date{2017年08月24日}
	
    %----A4设置----%
    \usepackage{geometry}
    \geometry{left=1cm,right=1cm,top=1cm,bottom=1cm}

    %数学包%
    \usepackage{amsmath}
    %页面分栏%
    \usepackage{multicol}

\begin{document}

    \begin{center}
        \Large 矩阵运算
    \end{center}

    \columnseprule=1pt
    \begin{multicols}{4}
    \end{multicols}

    矩阵定义:
    \[
        P = 2 , A =
        \begin{bmatrix}
            1 & 2 & 3 \\
            1 & 2 & 3 \\
            1 & 2 & 3
        \end{bmatrix}
        , B =
        \begin{bmatrix}
            3 & 2 & 1 \\
            3 & 2 & 1 \\
            3 & 2 & 1
        \end{bmatrix}
        , C =
        \begin{bmatrix}
            1 & 2 & 3
        \end{bmatrix}
        , D =
        \begin{bmatrix}
            1\\
            2\\
            3
        \end{bmatrix}
        , E =
        \begin{bmatrix}
            2
        \end{bmatrix}
    \]
    
    矩阵转置:
    \[
        A^T =
        \begin{bmatrix}
            1 & 1 & 1 \\
            2 & 2 & 2 \\
            3 & 3 & 3
        \end{bmatrix}
        , B^T =
        \begin{bmatrix}
            3 & 3 & 3 \\
            2 & 2 & 2 \\
            1 & 1 & 1
        \end{bmatrix}
        , C^T =
        \begin{bmatrix}
            1 \\
            2 \\
            3
        \end{bmatrix}
        , D^T =
        \begin{bmatrix}
            1 & 2 & 3
        \end{bmatrix}
        , E^T =
        \begin{bmatrix}
            2
        \end{bmatrix}
    \]

    常数运算:
    \[ \begin{split}
        A + P =
        \begin{bmatrix}
            3 & 4 & 5 \\
            3 & 4 & 5 \\
            3 & 4 & 5
        \end{bmatrix}
        , A - P =
        \begin{bmatrix}
            -1 & 0 & 1 \\
            -1 & 0 & 1 \\
            -1 & 0 & 1
        \end{bmatrix}
        , A \times\; P =
        \begin{bmatrix}
            2 & 4 & 6 \\
            2 & 4 & 6 \\
            2 & 4 & 6
        \end{bmatrix}
        , A \div\; P =
        \begin{bmatrix}
            0.50 & 1 & 1.5 \\
            0.50 & 1 & 1.5 \\
            0.50 & 1 & 1.5
        \end{bmatrix}
        \\
        P + A =
        \begin{bmatrix}
            3 & 4 & 5 \\
            3 & 4 & 5 \\
            3 & 4 & 5
        \end{bmatrix}
        , P - A =
        \begin{bmatrix}
            1 & 0 & -1 \\
            1 & 0 & -1 \\
            1 & 0 & -1
        \end{bmatrix}
        , P \times\; A =
        \begin{bmatrix}
            2 & 4 & 6 \\
            2 & 4 & 6 \\
            2 & 4 & 6
        \end{bmatrix}
        , P \div\; A =
        \begin{bmatrix}
            2 & 1.0 & 0.66 \\
            2 & 1.0 & 0.66 \\
            2 & 1.0 & 0.66
        \end{bmatrix}
    \end{split} \]

    \[ \begin{split}
        C + P =
        \begin{bmatrix}
            3 & 4 & 5
        \end{bmatrix}
        , C - P =
        \begin{bmatrix}
            -1 & 0 & 1
        \end{bmatrix}
        , C \times\; P =
        \begin{bmatrix}
            2 & 4 & 6
        \end{bmatrix}
        , C \div\; P =
        \begin{bmatrix}
            0.50 & 1 & 1.5
        \end{bmatrix}
        \\
        P + C =
        \begin{bmatrix}
            3 & 4 & 5
        \end{bmatrix}
        , P - C =
        \begin{bmatrix}
            1 & 0 & -1
        \end{bmatrix}
        , P \times\; C =
        \begin{bmatrix}
            2 & 4 & 6
        \end{bmatrix}
        , P \div\; C =
        \begin{bmatrix}
            2 & 1.0 & 0.66
        \end{bmatrix}
    \end{split} \]

    \[ \begin{split}
        D + P =
        \begin{bmatrix}
            3 \\
            4 \\
            5
        \end{bmatrix}
        , D - P =
        \begin{bmatrix}
            -1 \\
            0 \\
            1
        \end{bmatrix}
        , D \times\; P =
        \begin{bmatrix}
            2 \\
            4 \\
            6
        \end{bmatrix}
        , D \div\; P =
        \begin{bmatrix}
            0.50 \\
            1 \\
            1.5
        \end{bmatrix}
        \\
        P + D =
        \begin{bmatrix}
            3 \\
            4 \\
            5
        \end{bmatrix}
        , P - D =
        \begin{bmatrix}
            1 \\
            0 \\
            -1
        \end{bmatrix}
        , P \times\; D =
        \begin{bmatrix}
            2 \\
            4 \\
            6
        \end{bmatrix}
        , P \div\; D =
        \begin{bmatrix}
            2 \\
            1 \\
            0.66
        \end{bmatrix}
    \end{split} \]

    矩阵运算:
    \[ \begin{split}
        A + B =
        \begin{bmatrix}
            4 & 4 & 4 \\
            4 & 4 & 4 \\
            4 & 4 & 4
        \end{bmatrix}
        , A - B =
        \begin{bmatrix}
            -2 & 0 & 2 \\
            -2 & 0 & 2 \\
            -2 & 0 & 2
        \end{bmatrix}
        , A \times\; B =
        \begin{bmatrix}
            18 & 12 & 6 \\
            18 & 12 & 6 \\
            18 & 12 & 6
        \end{bmatrix}
        , A \div\; B =
        \begin{bmatrix}
            0.33 & 1 & 3 \\
            0.33 & 1 & 3 \\
            0.33 & 1 & 3
        \end{bmatrix}
        \\
        B + A =
        \begin{bmatrix}
            4 & 4 & 4 \\
            4 & 4 & 4 \\
            4 & 4 & 4
        \end{bmatrix}
        , B - A =
        \begin{bmatrix}
            2 & 0 & -2 \\
            2 & 0 & -2 \\
            2 & 0 & -2
        \end{bmatrix}
        , B \times\; A =
        \begin{bmatrix}
            6 & 12 & 18 \\
            6 & 12 & 18 \\
            6 & 12 & 18
        \end{bmatrix}
        , B \div\; A =
        \begin{bmatrix}
            3 & 1 & 0.33 \\
            3 & 1 & 0.33 \\
            3 & 1 & 0.33
        \end{bmatrix}
    \end{split} \]

    \[ \begin{split}
        A + C =
        \begin{bmatrix}
            2 & 4 & 6 \\
            2 & 4 & 6 \\
            2 & 4 & 6
        \end{bmatrix}
        , A - C =
        \begin{bmatrix}
            0 & 0 & 0 \\
            0 & 0 & 0 \\
            0 & 0 & 0
        \end{bmatrix}
        , A \times\; C =
        \begin{bmatrix}
            ERROR
        \end{bmatrix}
        , A \div\; C =
        \begin{bmatrix}
            1 & 1 & 1 \\
            1 & 1 & 1 \\
            1 & 1 & 1
        \end{bmatrix}
        \\
        C + A =
        \begin{bmatrix}
            2 & 4 & 6 \\
            2 & 4 & 6 \\
            2 & 4 & 6
        \end{bmatrix}
        , C - A =
        \begin{bmatrix}
            0 & 0 & 0 \\
            0 & 0 & 0 \\
            0 & 0 & 0
        \end{bmatrix}
        , C \times\; A =
        \begin{bmatrix}
            6 & 12 & 18
        \end{bmatrix}
        , C \div\; A =
        \begin{bmatrix}
            1 & 1 & 1 \\
            1 & 1 & 1 \\
            1 & 1 & 1
        \end{bmatrix}
    \end{split} \]

    \[ \begin{split}
        A + D =
        \begin{bmatrix}
            2 & 3 & 4 \\
            3 & 4 & 5 \\
            4 & 5 & 6
        \end{bmatrix}
        , A - D =
        \begin{bmatrix}
             0 & 1 & 2 \\
            -1 & 0 & 1 \\
            -2 & 1 & 0
        \end{bmatrix}
        , A \times\; D =
        \begin{bmatrix}
            \quad 14 \quad\quad \\
            \quad 14 \quad\quad \\
            \quad 14 \quad\quad
        \end{bmatrix}
        , A \div\; D =
        \begin{bmatrix}
            1    & 2    & 3   \\
            0.50 & 1    & 1.5 \\
            0.33 & 0.66 & 1
        \end{bmatrix}
        \\
        D + A =
        \begin{bmatrix}
            2 & 3 & 4 \\
            3 & 4 & 5 \\
            4 & 5 & 6
        \end{bmatrix}
        , D - A =
        \begin{bmatrix}
             0 & -1 & -2 \\
             1 &  0 & -1 \\
             2 &  1 &  0
        \end{bmatrix}
        , D \times\; A =
        \begin{bmatrix}
            ERROR
        \end{bmatrix}
        , D \div\; A =
        \begin{bmatrix}
            1.0 & 0.50  & 0.33 \\
            2   & 1     & 0.66 \\
            3   & 1.5   & 1
        \end{bmatrix}
    \end{split} \]

    \[ \begin{split}
        A + E =
        \begin{bmatrix}
            3 & 4 & 5 \\
            3 & 4 & 5 \\
            3 & 4 & 5
        \end{bmatrix}
        , A - E =
        \begin{bmatrix}
            -1 & 0 & 1 \\
            -1 & 0 & 1 \\
            -1 & 0 & 1
        \end{bmatrix}
        , A \times\; E =
        \begin{bmatrix}
            ERROR
        \end{bmatrix}
        , A \div\; E =
        \begin{bmatrix}
            0.50 & 1 & 1.5 \\
            0.5  & 1 & 1.5 \\
            0.5  & 1 & 1.5
        \end{bmatrix}
        \\
        E + A =
        \begin{bmatrix}
            3 & 4 & 5 \\
            3 & 4 & 5 \\
            3 & 4 & 5
        \end{bmatrix}
        , E - A =
        \begin{bmatrix}
            1 & 0 & -1 \\
            1 & 0 & -1 \\
            1 & 0 & -1
        \end{bmatrix}
        , E \times\; A =
        \begin{bmatrix}
            ERROR
        \end{bmatrix}
        , E \div\; A =
        \begin{bmatrix}
            2.0 & 1 & 0.66 \\
            2   & 1 & 0.66 \\
            2   & 1 & 0.66
        \end{bmatrix}
    \end{split} \]

    \[ \begin{split}
        C + D =
        \begin{bmatrix}
            2 & 3 & 4 \\
            3 & 4 & 5 \\
            4 & 5 & 6
        \end{bmatrix}
        , C - D =
        \begin{bmatrix}
             0 &  1 & 2 \\
            -1 &  0 & 1 \\
            -2 & -1 & 0
        \end{bmatrix}
        , C \times\; D =
        \begin{bmatrix}
            \quad 14 \quad\quad
        \end{bmatrix}
        , C \div\; D =
        \begin{bmatrix}
            1    & 2    & 3   \\
            0.5  & 1    & 1.50 \\
            0.33 & 0.66 & 1
        \end{bmatrix}
        \\
        D + C =
        \begin{bmatrix}
            2 & 3 & 4 \\
            3 & 4 & 5 \\
            4 & 5 & 6
        \end{bmatrix}
        , D - C =
        \begin{bmatrix}
            0 & -1 & -2 \\
            1 &  0 & -1 \\
            2 &  1 &  0
        \end{bmatrix}
        , D \times\; C =
        \begin{bmatrix}
            1 & 2 & 3 \\
            2 & 4 & 6 \\
            3 & 6 & 9
        \end{bmatrix}
        , D \div\; C =
        \begin{bmatrix}
            1.00 & 0.50 & 0.33 \\
            2   & 1    & 0.66 \\
            3   & 1.5  & 1
        \end{bmatrix}
    \end{split} \]
    
    源码示例:
    \begin{verbatim}
        import numpy as nm
        P=2
        A=nm.mat([[1,2,3],[1,2,3],[1,2,3]])
        B=nm.mat([[3,2,1],[3,2,1],[3,2,1]])
        C=nm.mat([[1,2,3]])
        D=nm.mat([[1],[2],[3]])
        E=nm.mat([[2]])
    \end{verbatim}

		
\end{document}
